Test/EUF/Distinct.lean
@@ -1,0 +1,9 @@
+import Smt
+
+example [Nonempty U] {a b c : U} (hab : a ≠ b) (hac : a ≠ c) (hbc : b ≠ c) :
+    distinctN [a, b, c] := by
+  smt_show [hab, hac, hbc]
+  exact ⟨hab, hac, hbc⟩
+
+example [Nonempty U] {a b c : U} (h : distinctN [a, b, c]) : a ≠ c := by
+  smt [h]
